SyBloc/SBWellDefined.v
@@ -207,6 +207,9 @@ Module Type SBWELLDEFINED
       + intro; apply Step; right; auto.
   Qed.
 
+  Module PN_as_OT := OrdersEx.PairOrderedType OrdersEx.Positive_as_OT OrdersEx.Nat_as_OT.
+  Module PNS := MSetList.Make PN_as_OT.
+
   Section Decide.
 
     Variable mems : PS.t.
@@ -262,7 +265,27 @@ Module Type SBWELLDEFINED
       destruct eq; simpl; split; try inversion_clear 1; auto using Is_state_in_eq.
     Qed.
 
-    Definition check_eq (eq: equation) (acc: bool * PS.t * PS.t * Env.t nat) : bool * PS.t * PS.t * Env.t nat :=
+    Definition check_state (s: ident) (k: nat) (sk: ident * nat) : bool :=
+      if ident_eqb (fst sk) s then NPeano.ltb (snd sk) k else true.
+
+    Lemma check_state_spec:
+      forall s k s' k',
+        check_state s k (s', k') = true
+        <->
+        (s = s' -> k' < k).
+    Proof.
+      intros; unfold check_state; simpl.
+      split.
+      - intros ** E Eq; subst.
+        rewrite ident_eqb_refl in E.
+        apply NPeano.ltb_lt; auto.
+      - intros Spec.
+        destruct (ident_eqb s' s) eqn: E; auto.
+        apply NPeano.ltb_lt, Spec.
+        symmetry; apply ident_eqb_eq; auto.
+    Qed.
+
+    Definition check_eq (eq: equation) (acc: bool * PS.t * PS.t * PNS.t) : bool * PS.t * PS.t * PNS.t :=
       match acc with
       | (true, defs, vars, states) =>
         let xs := defined_eq eq in
@@ -272,26 +295,23 @@ Module Type SBWELLDEFINED
         let vars := variables_eq vars eq in
         match state_eq eq with
         | Some (s, k) =>
-          (match Env.find s states with
-           | Some k' => NPeano.ltb k' k && b
-           | None => b
-           end,
-           defs, vars, Env.add s k states)
+          (PNS.for_all (check_state s k) states && b,
+           defs, vars, PNS.add (s, k) states)
         | None => (b, defs, vars, states)
         end
-      | (false, _, _, _) => (false, PS.empty, PS.empty, Env.empty _)
+      | (false, _, _, _) => (false, PS.empty, PS.empty, PNS.empty)
       end.
 
     Definition well_sch (args: idents) (eqs: list equation) : bool :=
       fst (fst (fst (fold_right check_eq (true,
                                           PS.empty,
                                           ps_from_list args,
-                                          Env.empty _) eqs))).
+                                          PNS.empty) eqs))).
 
-    Lemma not_for_all_spec:
+    Lemma PS_not_for_all_spec:
       forall (s : PS.t) (f : BinNums.positive -> bool),
         SetoidList.compat_bool PS.E.eq f ->
-        (PS.for_all f s = false <-> ~(PS.For_all (fun x : PS.elt => f x = true) s)).
+        (PS.for_all f s = false <-> ~ PS.For_all (fun x => f x = true) s).
     Proof.
       intros s f HSL.
       split.
@@ -306,14 +326,37 @@ Module Type SBWELLDEFINED
         assumption.
     Qed.
 
-    Lemma check_var_compat:
-      forall defined variables,
-        SetoidList.compat_bool PS.E.eq (check_var defined variables).
+    Lemma pair_eq:
+      forall A B (x y: A * B),
+        RelationPairs.RelProd Logic.eq Logic.eq x y <-> x = y.
     Proof.
-      intros defined variables x y Heq.
-      unfold PS.E.eq in Heq.
-      rewrite Heq.
-      reflexivity.
+      split; intros ** E; subst; auto.
+      destruct x, y.
+      inversion_clear E as [Fst Snd]; inv Fst; inv Snd; simpl in *; subst; auto.
+    Qed.
+
+    Lemma PNS_compat:
+      forall A (f: (positive * nat) -> A),
+        Morphisms.Proper (Morphisms.respectful (RelationPairs.RelProd Logic.eq Logic.eq) Logic.eq) f.
+    Proof.
+      intros ** x y E.
+      apply pair_eq in E; subst; auto.
+    Qed.
+    Hint Resolve PNS_compat.
+
+    Lemma PNS_not_for_all_spec:
+      forall (s : PNS.t) (f : positive * nat -> bool),
+        PNS.for_all f s = false <-> ~ PNS.For_all (fun x => f x = true) s.
+    Proof.
+      split.
+      - intros Hfa HFa.
+        apply PNS.for_all_spec in HFa; auto.
+        rewrite Hfa in HFa.
+        discriminate.
+      - intro HFa.
+        apply Bool.not_true_iff_false.
+        intro Hfa; apply HFa.
+        apply PNS.for_all_spec; auto.
     Qed.
 
     (* Lemma in_fold_left_add: *)
@@ -333,18 +376,123 @@ Module Type SBWELLDEFINED
     (*   - simpl; apply IH; simpl in H; intuition. *)
     (* Qed. *)
 
+    Lemma free_spec:
+      forall eqs args defs vars eq x,
+        (forall x, PS.In x defs <-> Is_defined_in x eqs) ->
+        (forall x, PS.In x vars <-> Is_variable_in x eqs \/ In x args) ->
+        PS.For_all (fun x => check_var defs vars x = true) (free_in_eq eq PS.empty) ->
+        Is_free_in_eq x eq ->
+        if PS.mem x mems then ~ Is_defined_in x eqs else Is_variable_in x eqs \/ In x args.
+    Proof.
+      intros ** DefSpec VarSpec E Hfree.
+      apply free_in_eq_spec', E, check_var_spec in Hfree as (Hin & Hnin).
+      destruct (PS.mem x mems) eqn: Mem.
+      - rewrite <-DefSpec; apply PSE.MP.Dec.F.mem_iff, Hin in Mem; auto.
+      - rewrite <-VarSpec; apply PSE.MP.Dec.F.not_mem_iff, Hnin in Mem; auto.
+    Qed.
+
+    Lemma def_spec:
+      forall eqs defs eq x,
+        (forall x, PS.In x defs <-> Is_defined_in x eqs) ->
+        existsb (fun x => PS.mem x defs) (defined_eq eq) = false ->
+        Is_defined_in_eq x eq ->
+        ~ Is_defined_in x eqs.
+    Proof.
+      intros ** DefSpec E Hdef Hdefs.
+      apply DefSpec in Hdefs; apply Is_defined_in_defined_eq in Hdef.
+      apply In_ex_nth with (d := Ids.default) in Hdef as (?&?&?); subst.
+      eapply existsb_nth with (d := Ids.default) in E; eauto.
+      apply PSE.MP.Dec.F.not_mem_iff in E; auto.
+    Qed.
+
+    Lemma check_var_compat:
+      forall defined variables,
+        SetoidList.compat_bool PS.E.eq (check_var defined variables).
+    Proof.
+      intros defined variables x y Heq.
+      unfold PS.E.eq in Heq.
+      rewrite Heq.
+      reflexivity.
+    Qed.
+    Hint Resolve check_var_compat.
+
+    Lemma not_well_sch_vars_defs_spec:
+      forall eqs args defs vars eq,
+         (forall x, PS.In x defs <-> Is_defined_in x eqs) ->
+         (forall x, PS.In x vars <-> Is_variable_in x eqs \/ In x args) ->
+         PS.for_all (check_var defs vars) (free_in_eq eq PS.empty) &&
+                 negb (existsb (fun x => PS.mem x defs) (defined_eq eq)) = false ->
+        ~ Is_well_sch args mems (eq :: eqs).
+    Proof.
+      intros ** DefSpec VarSpec E Wsch.
+      inversion_clear Wsch as [|??? Hfree Hdefs].
+      apply Bool.andb_false_iff in E as [E|E].
+      - apply PS_not_for_all_spec in E; auto.
+        apply E; intros x Hin; apply free_in_eq_spec' in Hin.
+        apply Hfree in Hin.
+        apply check_var_spec; split.
+        + rewrite PSE.MP.Dec.F.mem_iff; intro Hin'; rewrite Hin' in Hin.
+          now rewrite DefSpec.
+        + rewrite PSE.MP.Dec.F.not_mem_iff; intro Hin'; rewrite Hin' in Hin.
+          now rewrite VarSpec.
+      - apply Bool.negb_false_iff, existsb_exists in E as (?& Hin & Hin').
+        apply Is_defined_in_defined_eq in Hin.
+        apply PSE.MP.Dec.F.mem_iff, DefSpec in Hin'.
+        eapply Hdefs; eauto.
+    Qed.
+
+    Lemma Is_defined_in_adds_defined_eq:
+      forall eqs defs eq x,
+        (forall x, PS.In x defs <-> Is_defined_in x eqs) ->
+        (PS.In x (ps_adds (defined_eq eq) defs) <-> Is_defined_in x (eq :: eqs)).
+    Proof.
+      intros ** DefSpec; split; intro Hin;
+        [apply ps_adds_spec in Hin as [|]|apply ps_adds_spec; inv Hin];
+        try (now left; apply Is_defined_in_defined_eq; auto);
+        try (now right; apply DefSpec; auto); auto.
+    Qed.
+
+    Lemma Is_variable_in_variables_eq:
+      forall eqs args vars eq x,
+        (forall x, PS.In x vars <-> Is_variable_in x eqs \/ In x args) ->
+        (PS.In x (variables_eq vars eq) <-> Is_variable_in x (eq :: eqs) \/ In x args).
+    Proof.
+      intros ** VarSpec; split; intro Hin.
+      - apply variables_eq_empty in Hin as [Hin|Hin].
+        + destruct eq; simpl in *; try (contradict Hin; apply not_In_empty).
+          *{ apply PSE.MP.Dec.F.add_iff in Hin as [|Hin]; subst.
+             - left; left; constructor.
+             - contradict Hin; apply not_In_empty.
+           }
+          *{ apply ps_adds_spec in Hin as [|Hin].
+             - left; left; constructor; auto.
+             - contradict Hin; apply not_In_empty.
+           }
+        + apply VarSpec in Hin as [|]; intuition.
+          left; right; auto.
+      - apply variables_eq_empty; destruct Hin as [Hin|].
+        + inversion_clear Hin as [?? Hin'|].
+          *{ destruct eq; simpl; inv Hin'.
+             - rewrite PSE.MP.Dec.F.add_iff; auto.
+             - rewrite ps_adds_spec; auto.
+           }
+          * rewrite VarSpec; auto.
+        + rewrite VarSpec; auto.
+    Qed.
+
+
     Lemma well_sch_pre_spec:
       forall args eqs ok defs vars states,
         fold_right check_eq (true,
                              PS.empty,
                              ps_from_list args,
-                             Env.empty _) eqs = (ok, defs, vars, states) ->
+                             PNS.empty) eqs = (ok, defs, vars, states) ->
         if ok
         then
           Is_well_sch args mems eqs
           /\ (forall x, PS.In x defs <-> Is_defined_in x eqs)
           /\ (forall x, PS.In x vars <-> Is_variable_in x eqs \/ In x args)
-          /\ (forall s k, Env.find s states = Some k <-> Is_state_in s k eqs)
+          /\ (forall s k, PNS.In (s, k) states <-> Is_state_in s k eqs)
         else
           ~Is_well_sch args mems eqs.
     Proof.
@@ -352,7 +500,7 @@ Module Type SBWELLDEFINED
       - simpl; inversion_clear 1; intuition; try (now constructor);
           repeat match goal with
                  | H:PS.In _ PS.empty |- _ => apply PS.empty_spec in H; contradiction
-                 | H:Env.find _ (Env.empty _) = _ |- _ => rewrite Env.gempty in H; discriminate
+                 | H:PNS.In _ PNS.empty |- _ => apply PNS.empty_spec in H; contradiction
                  | H:Is_defined_in _ nil |- _ => inversion H
                  | H:Is_variable_in _ nil |- _ => inversion H
                  | H:Is_state_in _ _ nil |- _ => inversion H
@@ -362,255 +510,96 @@ Module Type SBWELLDEFINED
                  end.
         apply ps_from_list_In; auto.
       - simpl; intros ** HH.
-        destruct (fold_right check_eq (true, PS.empty, ps_from_list args, Env.empty nat) eqs)
+        destruct (fold_right check_eq (true, PS.empty, ps_from_list args, PNS.empty) eqs)
           as [[[ok' defs'] vars'] states'].
         specialize (IHeqs ok' defs'  vars' states' eq_refl).
         simpl in HH.
         destruct ok'.
         + destruct IHeqs as (Wsch & DefSpec & VarSpec & StateSpec).
-          destruct (state_eq eq) eqn: St.
-          * admit.
-          *{ destruct ok; inversion HH as [E]; [apply Bool.andb_true_iff in E as (E & E')|].
-             - apply PS.for_all_spec in E; try now apply check_var_compat.
-               apply Bool.negb_true_iff in E'.
-               split; [|split; [|split]].
+          assert (forall x, PS.In x (ps_adds (defined_eq eq) defs') <-> Is_defined_in x (eq :: eqs))
+            by (intros; eapply Is_defined_in_adds_defined_eq; eauto).
+          assert (forall x, PS.In x (variables_eq vars' eq) <-> Is_variable_in x (eq :: eqs) \/ In x args)
+            by (intros; eapply Is_variable_in_variables_eq; eauto).
+          destruct (state_eq eq) as [(s, k)|] eqn: St.
+          *{ destruct ok; inversion HH as [E]; clear HH.
+             - apply Bool.andb_true_iff in E as (E & E');
+                 apply Bool.andb_true_iff in E' as (E' & E'').
+               apply PNS.for_all_spec in E; auto.
+               apply PS.for_all_spec in E'; auto.
+               apply Bool.negb_true_iff in E''.
+               split; [|split; [|split]]; auto.
                + constructor; auto.
-                 *{ intros ** Hfree.
-                    apply free_in_eq_spec', E, check_var_spec in Hfree as (Hin & Hnin).
-                    destruct (PS.mem x mems) eqn: Mem.
-                    - rewrite <-DefSpec; apply PSE.MP.Dec.F.mem_iff, Hin in Mem; auto.
-                    - rewrite <-VarSpec; apply PSE.MP.Dec.F.not_mem_iff, Hnin in Mem; auto.
+                 * intros; eapply free_spec; eauto.
+                 * intros; eapply def_spec; eauto.
+                 * intros ** Hin; apply Is_state_in_state_eq in Hin; rewrite Hin in St; inv St.
+                   apply Forall_forall; intros.
+                   assert (Is_state_in s k' eqs) as Hst
+                       by (apply Exists_exists; eexists; intuition; eauto).
+                   apply StateSpec in Hst; apply E in Hst.
+                   apply check_state_spec in Hst; auto.
+               + rewrite <-Is_state_in_state_eq in St.
+                 intros s' k'; split; rewrite PNS.add_spec.
+                 *{ intros [Eq|Hin].
+                    - apply pair_eq in Eq; inv Eq; left; auto.
+                    - apply StateSpec in Hin; right; auto.
                   }
-                 * setoid_rewrite <-DefSpec; setoid_rewrite Is_defined_in_defined_eq.
-                   intros x Hin.
-                   apply In_ex_nth with (d := Ids.default) in Hin as (?&?&?); subst.
-                   eapply existsb_nth with (d := Ids.default) in E'; eauto.
-                   now apply PSE.MP.Dec.F.not_mem_iff.
-                 * setoid_rewrite Is_state_in_state_eq; rewrite St; discriminate.
-               + intro x; split; intro Hin;
-                   [apply ps_adds_spec in Hin as [|]|apply ps_adds_spec; inv Hin];
-                   try (now left; apply Is_defined_in_defined_eq; auto);
-                   try (now right; apply DefSpec; auto); auto.
-               + intro x; split; intro Hin.
-                 *
-                 (* variables set *)
-            intro x; split; intro HH.
-            apply variable_eq_empty in HH.
-            destruct HH as [HH|HH].
-            destruct eq;
-              match goal with
-              | |- context[ EqApp _ _ _ _ ] =>
-                generalize ps_adds_spec; intro add_spec
-              | _ =>
-                generalize PS.add_spec; intro add_spec
-              end;
-              ((apply add_spec in HH;
-                destruct HH as [HH|HH];
-                [try subst i; left; now repeat constructor
-                |apply PS.empty_spec in HH; contradiction])
-               || apply PS.empty_spec in HH; contradiction).
-            apply IHvar in HH; intuition; left; constructor (assumption).
-            apply variable_eq_empty.
-            destruct HH as [HH|HH].
-            apply Is_variable_in_cons in HH.
-            destruct HH as [HH|HH]; [left|right].
-            destruct eq;
-              match goal with
-              | |- context[ EqApp _ _ _ _ ] =>
-                generalize ps_adds_spec; intro add_spec
-              | _ =>
-                generalize PS.add_spec; intro add_spec
-              end;
-              inversion_clear HH; simpl;
-                try (rewrite add_spec; auto);
-                intuition.
-            apply IHvar; intuition.
-            right; apply IHvar; auto.
+                 *{ rewrite pair_eq; inversion_clear 1 as [?? St'|].
+                    - inv St; inv St'; auto.
+                    - right; apply StateSpec; auto.
+                  }
 
-               SearchAbout (_ && _) true. inv HH.
+             - apply Bool.andb_false_iff in E as [E|];
+                 [|eapply not_well_sch_vars_defs_spec; eauto].
+               inversion_clear 1 as [|????? Hstates].
+               rewrite <-Is_state_in_state_eq in St.
+               apply Hstates in St.
+               apply PNS_not_for_all_spec in E; apply E; clear E.
+               intros (s', k') Hin.
+               apply check_state_spec; intros; subst.
+               apply StateSpec in Hin.
+               eapply Forall_Exists, Exists_exists in Hin as (?&?& Spec & St'); eauto; auto.
+           }
+          *{ destruct ok; inversion HH as [E].
+             - apply Bool.andb_true_iff in E as (E & E').
+               apply PS.for_all_spec in E; try apply check_var_compat.
+               apply Bool.negb_true_iff in E'.
+               split; [|split; [|split]]; auto.
+               + constructor; auto.
+                 * intros; eapply free_spec; eauto.
+                 * intros; eapply def_spec; eauto.
+                 * intros ** Hin; apply Is_state_in_state_eq in Hin; rewrite Hin in St; inv St.
+               + subst; setoid_rewrite StateSpec.
+                 split.
+                 * right; auto.
+                 * rewrite <-not_Some_is_None in St.
+                   specialize (St (s, k)).
+                   rewrite <-Is_state_in_state_eq in St.
+                   inversion 1; auto; contradiction.
+             - eapply not_well_sch_vars_defs_spec; eauto.
+           }
 
-        + inv HH.
-          inversion_clear 1; contradiction.
-
-
-
-
-          simpl in HH.
-        destruct IH as [IHt IHf].
-        split; intro Hg; rewrite Hg in *; clear Hg.
-        + (* good=true *)
-          simpl in HH; rewrite Heq in HH.
-          simpl in HH.
-          destruct good'; [|discriminate].
-          specialize (IHt eq_refl).
-          clear IHf; destruct IHt as [IHwsch [IHdef IHvar]].
-          injection HH; clear HH; intros Hv Hd H.
-          subst variables; subst defined.
-          symmetry in H.
-          apply Bool.andb_true_iff in H.
-          destruct H as [H1 H2].
-          apply PS.for_all_spec in H1; [|now apply check_var_compat].
-          apply Bool.negb_true_iff in H2.
-
-          assert (forall x, In x (var_defined eq) -> ~ PS.In x defined')
-            as Hnot_def.
-          {
-            intros x Hin.
-
-            assert (exists n,
-                       n < length (var_defined eq)
-                     /\ nth n (var_defined eq) Ids.default = x)
-              as (n & Hlen & Hnth)
-                by now apply In_ex_nth.
-
-            assert (PS.mem x defined' = false)
-              by now subst x;
-                     eapply existsb_nth
-                       with (f := (fun x => PS.mem x defined')).
-
-            now apply mem_spec_false.
-          }
-
-          split; [|split].
-          * (* Is_well_sch *)
-            assert (forall i,
-                       IsF.Is_free_in_eq i eq ->
-                       (PS.In i mems -> ~ Is_defined_in_eqs i eqs) /\
-                       (~ PS.In i mems -> Is_variable_in_eqs i eqs \/ In i args)).
-            {
-              intros x Hfree.
-              apply free_in_equation_spec' in Hfree.
-              apply H1 in Hfree.
-              apply check_var_spec in Hfree.
-              destruct Hfree as [Hfree1 Hfree2].
-              split; intro HH; (apply Hfree1 in HH || apply Hfree2 in HH).
-              - now intro; apply HH; apply IHdef.
-              - now apply IHvar.
-            }
-
-            assert (forall i, Is_defined_in_eq i eq -> ~ Is_defined_in_eqs i eqs).
-            {
-              intros x Hdef Hdefs; apply IHdef in Hdefs.
-              apply Is_defined_in_eqs_var_defined in Hdef.
-              now eapply Hnot_def; eauto.
-            }
-
-            now constructor.
-          * (* defined set *)
-            intro x; split; intro HH.
-            apply ps_adds_spec in HH.
-            destruct HH as [HH|HH].
-            constructor; now apply Is_defined_in_eqs_var_defined.
-            apply IHdef in HH.
-            constructor (assumption).
-            apply ps_adds_spec.
-            inversion_clear HH.
-            apply Is_defined_in_eqs_var_defined in H; auto.
-            right; apply IHdef; assumption.
-          * (* variables set *)
-            intro x; split; intro HH.
-            apply variable_eq_empty in HH.
-            destruct HH as [HH|HH].
-            destruct eq;
-              match goal with
-              | |- context[ EqApp _ _ _ _ ] =>
-                generalize ps_adds_spec; intro add_spec
-              | _ =>
-                generalize PS.add_spec; intro add_spec
-              end;
-              ((apply add_spec in HH;
-                destruct HH as [HH|HH];
-                [try subst i; left; now repeat constructor
-                |apply PS.empty_spec in HH; contradiction])
-               || apply PS.empty_spec in HH; contradiction).
-            apply IHvar in HH; intuition; left; constructor (assumption).
-            apply variable_eq_empty.
-            destruct HH as [HH|HH].
-            apply Is_variable_in_cons in HH.
-            destruct HH as [HH|HH]; [left|right].
-            destruct eq;
-              match goal with
-              | |- context[ EqApp _ _ _ _ ] =>
-                generalize ps_adds_spec; intro add_spec
-              | _ =>
-                generalize PS.add_spec; intro add_spec
-              end;
-              inversion_clear HH; simpl;
-                try (rewrite add_spec; auto);
-                intuition.
-            apply IHvar; intuition.
-            right; apply IHvar; auto.
-        + (* good=false *)
-          intro Hwsch.
-          simpl in HH; rewrite Heq in HH; clear Heq; simpl in HH.
-          destruct good'; [specialize (IHt eq_refl); clear IHf
-                          | specialize (IHf eq_refl);
-                            apply Is_well_sch_cons in Hwsch;
-                            apply IHf with (1:=Hwsch)].
-          destruct IHt as [_ [IHdef IHvar]].
-          injection HH; clear HH; intros Hv Hd HH.
-          subst variables; subst defined; symmetry in HH.
-          apply Bool.andb_false_iff in HH.
-          inversion_clear Hwsch as [|Ha Hb Hwschs Hfree Hdefd].
-          destruct HH as [HH|HH].
-          * (* check_var of free fails *)
-            apply not_for_all_spec in HH; [|apply check_var_compat].
-            apply HH; clear HH.
-            intros x HH.
-            apply free_in_equation_spec in HH.
-            destruct HH as [HH|HH]; [|apply PS.empty_spec in HH].
-            apply Hfree in HH.
-            destruct HH as [Hmem Hvar];
-              apply check_var_spec; split; intro HHm;
-                (specialize (Hmem HHm) || specialize (Hvar HHm)).
-            intro Hdef; apply IHdef in Hdef; apply Hmem; assumption.
-            apply IHvar; intuition.
-            contradiction.
-          * (* already defined *)
-            apply Bool.negb_false_iff in HH.
-
-            assert (exists x, In x (var_defined eq) /\ PS.In x defined')
-              as (x & Hdef & Hdef').
-            {
-              apply existsb_exists in HH.
-              destruct HH as (x & Hvar_def & Hmem).
-              rewrite PS.mem_spec in Hmem.
-              now eexists; eauto.
-            }
-
-            assert (Is_defined_in_eq x eq)
-              by now apply Is_defined_in_eqs_var_defined.
-
-            assert (Is_defined_in_eqs x eqs)
-              by now apply IHdef.
-
-            eapply Hdefd; now eauto.
+        + inv HH; inversion 1; auto.
     Qed.
 
     Lemma well_sch_spec:
       forall args eqns,
         if well_sch args eqns
-        then Is_well_sch mems args eqns
-        else ~Is_well_sch mems args eqns.
+        then Is_well_sch args mems eqns
+        else ~ Is_well_sch args mems eqns.
     Proof.
       intros args eqns.
-      pose proof (well_sch_pre_spec args eqns).
+      pose proof (well_sch_pre_spec args eqns) as Spec.
       unfold well_sch.
       destruct (fold_right check_eq
-                  (true, PS.empty,
-                   fold_left (fun a b => PS.add b a) args PS.empty) eqns)
-        as [[good defined] variables].
-      simpl.
-      specialize H with good defined variables.
-      pose proof (H (eq_refl _)) as H'; clear H.
-      destruct H' as [Ht Hf].
-      destruct good;
-        intuition.
+                  (true, PS.empty, ps_from_list args, PNS.empty) eqns)
+        as [[[ok defs] vars] states]; simpl.
+      specialize (Spec ok defs vars states eq_refl).
+      destruct ok; intuition.
     Qed.
 
     Lemma Is_well_sch_by_refl:
       forall args eqns,
-        well_sch args eqns = true <-> Is_well_sch mems args eqns.
+        well_sch args eqns = true <-> Is_well_sch args mems eqns.
     Proof.
       intros args eqns.
       pose proof (well_sch_spec args eqns) as Hwss.
@@ -622,7 +611,7 @@ Module Type SBWELLDEFINED
 
     Lemma well_sch_dec:
       forall args eqns,
-        {Is_well_sch mems args eqns}+{~Is_well_sch mems args eqns}.
+        {Is_well_sch args mems eqns} + {~ Is_well_sch args mems eqns}.
     Proof.
       intros args eqns.
       pose proof (well_sch_spec args eqns) as Hwss.
