SyBloc/SBSchedule.v
@@ -1,0 +1,442 @@
+Require Import List.
+Import List.ListNotations.
+Open Scope list_scope.
+Require Import Coq.Sorting.Permutation.
+Require Import Coq.Sorting.Mergesort.
+
+Require Import Coq.FSets.FMapPositive.
+Require Import Velus.Common.
+Require Import Velus.Operators.
+Require Import Velus.Clocks.
+Require Import Velus.NLustre.NLExprSyntax.
+Require Import Velus.SyBloc.SBSyntax.
+Require Import Velus.SyBloc.SBIsBlock.
+Require Import Velus.SyBloc.SBOrdered.
+Require Import Velus.NLustre.Stream.
+Require Import Velus.NLustre.NLExprSemantics.
+Require Import Velus.SyBloc.SBSemantics.
+
+Require Import RMemory.
+
+(** * Scheduling of N-Lustre equations *)
+
+(**
+
+  The scheduler routines are parameterized over an external scheduler
+  (EXT_NLSCHEDULER) that provides a schedule function.
+
+  The schedule function should map a list of equations to a list of priority
+  values (positive integers). If the output list has the same length as the
+  input list, the equations are sorted in ascending order of their priorities.
+
+  The idea is to allow an external scheduler to be written in OCaml. The
+  scheduler should order the equations by their dependencies. If this is
+  impossible, it should print an explanatory error message and return the
+  empty list.
+
+ *)
+
+Module Type EXT_NLSCHEDULER
+       (Import Ids    : IDS)
+       (Import Op     : OPERATORS)
+       (Import Clks   : CLOCKS   Ids)
+       (Import ExprSyn: NLEXPRSYNTAX Op)
+       (Import Syn    : SBSYNTAX Ids Op Clks ExprSyn).
+
+  Parameter schedule : ident -> list equation -> list positive.
+
+End EXT_NLSCHEDULER.
+
+Module Type SBSCHEDULE
+       (Import Ids    : IDS)
+       (Import Op     : OPERATORS)
+       (Import OpAux  : OPERATORS_AUX       Op)
+       (Import Clks   : CLOCKS          Ids)
+       (Import ExprSyn: NLEXPRSYNTAX        Op)
+       (Import Syn    : SBSYNTAX        Ids Op       Clks ExprSyn)
+       (Import Block  : SBISBLOCK       Ids Op       Clks ExprSyn Syn)
+       (Import Ord    : SBORDERED       Ids Op       Clks ExprSyn Syn Block)
+       (Import Str    : STREAM              Op OpAux)
+       (Import ExprSem: NLEXPRSEMANTICS Ids Op OpAux Clks ExprSyn               Str)
+       (Import Sem    : SBSEMANTICS     Ids Op OpAux Clks ExprSyn Syn Block Ord Str ExprSem)
+       (Import Sch    : EXT_NLSCHEDULER Ids Op       Clks ExprSyn Syn).
+
+  Section OCombine.
+    Context {A B: Type}.
+
+    Fixpoint ocombine (l : list A) (l' : list B) : option (list (A * B)) :=
+      match l, l' with
+      | [], [] => Some []
+      | x::xs, y::ys =>
+        match ocombine xs ys with
+        | None => None
+        | Some rs => Some ((x, y) :: rs)
+        end
+      | _, _ => None
+      end.
+
+    Lemma ocombine_combine:
+      forall l l' ll,
+        ocombine l l' = Some ll ->
+        combine l l' = ll.
+    Proof.
+      induction l, l'; simpl;
+        try (now inversion_clear 1; auto).
+      intros ** HH; cases_eqn Hoc; inv HH.
+      erewrite IHl; eauto.
+    Qed.
+
+    Lemma ocombine_length:
+      forall l l' ll,
+        ocombine l l' = Some ll ->
+        length l = length l'.
+    Proof.
+      induction l, l'; simpl; inversion 1; auto.
+      destruct (ocombine l l') eqn:Hoc.
+      now rewrite (IHl _ _ Hoc).
+      inv H.
+    Qed.
+
+  End OCombine.
+
+  Module SchEqOrder <: Orders.TotalLeBool'.
+
+    Definition t : Type := (positive * equation)%type.
+
+    (* The arguments are inversed to put the list in the reverse order
+       expected by [Is_well_sch]. *)
+    Definition leb (s1 s2 : t) : bool := ((fst s2) <=? (fst s1))%positive.
+
+    Lemma leb_total:
+      forall s1 s2,
+        leb s1 s2 = true \/ leb s2 s1 = true.
+    Proof.
+      destruct s1 as (p1 & eq1).
+      destruct s2 as (p2 & eq2).
+      unfold leb; simpl.
+      setoid_rewrite POrderedType.Positive_as_OT.leb_compare.
+      destruct (p1 ?= p2)%positive eqn:Hp; auto.
+      apply Pos.compare_gt_iff in Hp.
+      apply Pos.compare_lt_iff in Hp.
+      rewrite Hp; auto.
+    Qed.
+
+  End SchEqOrder.
+
+  Module SchSort := Sort SchEqOrder.
+
+  Definition schedule_eqs (f : ident) (eqs : list equation) : list equation :=
+    let sch := Sch.schedule f eqs in
+    match ocombine sch eqs with
+    | None => eqs
+    | Some scheqs =>
+      map snd (SchSort.sort scheqs)
+    end.
+
+  Lemma schedule_eqs_permutation:
+    forall f eqs,
+      Permutation (schedule_eqs f eqs) eqs.
+  Proof.
+    unfold schedule_eqs.
+    intros f eqs.
+    destruct (ocombine (schedule f eqs) eqs) eqn:Hoc; auto.
+    rewrite <-SchSort.Permuted_sort.
+    pose proof (ocombine_length _ _ _ Hoc) as Hlen.
+    apply ocombine_combine in Hoc.
+    rewrite <-Hoc, map_snd_combine; auto.
+  Qed.
+
+  Require Import Morphisms.
+  Require Import Setoid.
+
+  Add Parametric Morphism : (calls_of)
+      with signature @Permutation equation ==> @Permutation (ident * ident)
+        as calls_of_permutation.
+  Proof.
+    induction 1; simpl; auto.
+    - cases; rewrite IHPermutation.
+    - cases; apply perm_swap.
+    - etransitivity; eauto.
+  Qed.
+
+  Add Parametric Morphism : (resets_of)
+      with signature @Permutation equation ==> @Permutation (ident * ident)
+        as resets_of_permutation.
+  Proof.
+    induction 1; simpl; auto.
+    - cases; rewrite IHPermutation.
+    - cases; apply perm_swap.
+    - etransitivity; eauto.
+  Qed.
+
+  Add Parametric Morphism : (lasts_of)
+      with signature @Permutation equation ==> @Permutation ident
+        as lasts_of_permutation.
+  Proof.
+    induction 1; simpl; auto.
+    - cases; rewrite IHPermutation.
+    - cases; apply perm_swap.
+    - etransitivity; eauto.
+  Qed.
+
+  Add Parametric Morphism : (variables)
+      with signature @Permutation equation ==> @Permutation ident
+        as variables_permutation.
+  Proof.
+    unfold variables, concatMap.
+    induction 1; simpl; auto.
+    - now rewrite IHPermutation.
+    - rewrite <-2 Permutation_app_assoc; apply Permutation_app_tail, Permutation_app_comm.
+    - etransitivity; eauto.
+  Qed.
+
+  Add Parametric Morphism A P: (Exists P)
+      with signature @Permutation A ==> Basics.impl
+        as Exists_permutation.
+  Proof.
+    induction 1; intros Ex; auto.
+    - inv Ex.
+      + now left.
+      + right; auto.
+    - inversion_clear Ex as [|?? Ex'].
+      + now right; left.
+      + inv Ex'.
+        * now left.
+        * now right; right.
+  Qed.
+
+  Add Parametric Morphism s k: (Is_state_in s k)
+      with signature @Permutation equation ==> Basics.impl
+        as Is_state_in_permutation.
+  Proof.
+    unfold Is_state_in; intros ** E St.
+    now rewrite <-E.
+  Qed.
+
+  Program Definition schedule_block (b: block) : block :=
+    {| b_name   := b.(b_name);
+       b_blocks := b.(b_blocks);
+       b_in     := b.(b_in);
+       b_vars   := b.(b_vars);
+       b_lasts  := b.(b_lasts);
+       b_out    := b.(b_out);
+       b_eqs    := schedule_eqs b.(b_name) b.(b_eqs);
+
+       b_ingt0              := b.(b_ingt0);
+       b_nodup              := b.(b_nodup);
+       b_nodup_lasts_blocks := b.(b_nodup_lasts_blocks);
+       b_good               := b.(b_good)
+    |}.
+  Next Obligation.
+    do 2 setoid_rewrite schedule_eqs_permutation at 1;
+      apply b_blocks_in_eqs.
+  Qed.
+  Next Obligation.
+    rewrite schedule_eqs_permutation; apply b_blocks_calls_of.
+  Qed.
+  Next Obligation.
+    rewrite schedule_eqs_permutation; apply b_lasts_in_eqs.
+  Qed.
+  Next Obligation.
+    rewrite schedule_eqs_permutation; apply b_vars_out_in_eqs.
+  Qed.
+  Next Obligation.
+    unfold Step_with_reset_in; rewrite schedule_eqs_permutation in *;
+      now apply b_no_single_reset.
+  Qed.
+  Next Obligation.
+    unfold Step_with_reset_in in H; rewrite schedule_eqs_permutation in H.
+    apply b_reset_in in H.
+    cases; rewrite schedule_eqs_permutation; auto.
+  Qed.
+  Next Obligation.
+    rewrite schedule_eqs_permutation; apply b_reset_incl.
+  Qed.
+
+  Definition schedule (P: program) : program :=
+    map schedule_block P.
+
+  Lemma schedule_block_name:
+    forall b, (schedule_block b).(b_name) = b.(b_name).
+  Proof. destruct b; auto. Qed.
+
+  Lemma schedule_map_name:
+    forall P,
+      map b_name (schedule P) = map b_name P.
+  Proof.
+    induction P as [|b]; auto.
+    destruct b; simpl.
+    now rewrite IHP.
+  Qed.
+
+  Lemma scheduler_find_block:
+    forall P P' f b,
+      find_block f P = Some (b, P') ->
+      find_block f (schedule P) = Some (schedule_block b, schedule P').
+  Proof.
+    induction P as [|bl]; [now inversion 1|].
+    intros ** Hfind.
+    simpl in *.
+    destruct (ident_eqb bl.(b_name) f); auto.
+    inv Hfind; auto.
+  Qed.
+
+  Lemma scheduler_find_block':
+    forall P f b P',
+      find_block f (schedule P) = Some (b, P') ->
+      exists bl P'',
+        find_block f P = Some (bl, P'')
+        /\ b = schedule_block bl
+        /\ P' = schedule P''.
+  Proof.
+    induction P as [|bl]; [now inversion 1|].
+    intros ** Hfind.
+    simpl in *.
+    destruct (ident_eqb bl.(b_name) f); eauto.
+    inv Hfind; eauto.
+  Qed.
+
+  (* Lemma scheduler_wt_equation: *)
+  (*   forall G vars eq, *)
+  (*     wt_equation G vars eq -> *)
+  (*     wt_equation (schedule G) vars eq. *)
+  (* Proof. *)
+  (*   induction G as [|n G IH]. *)
+  (*   - now destruct eq; inversion_clear 1; eauto with nltyping. *)
+  (*   - destruct eq; inversion_clear 1; eauto with nltyping; *)
+  (*       match goal with H:find_node _ _ = _ |- _ => *)
+  (*                       apply scheduler_find_node in H end; *)
+  (*       destruct n0; eauto with nltyping. *)
+  (* Qed. *)
+
+  (* Lemma scheduler_wt_global: *)
+  (*   forall G, *)
+  (*     wt_global G -> *)
+  (*     wt_global (schedule G). *)
+  (* Proof. *)
+  (*   intros G HG. *)
+  (*   induction G as [|n G Hwt IH]; auto. *)
+  (*   inv HG. simpl. *)
+  (*   apply wtg_cons; auto. *)
+  (*   - unfold wt_node in *. *)
+  (*     destruct n; simpl in *. *)
+  (*     rewrite schedule_eqs_permutation. *)
+  (*     eapply Forall_impl with (2:=H2). *)
+  (*     apply scheduler_wt_equation. *)
+  (*   - change (Forall (fun n'=> *)
+  (*                       (fun x => n_name (schedule_node n) <> x) n'.(n_name)) *)
+  (*                    (schedule G)). *)
+  (*     rewrite <-Forall_map. *)
+  (*     rewrite schedule_map_name. *)
+  (*     rewrite Forall_map. *)
+  (*     destruct n; auto. *)
+  (* Qed. *)
+
+  (* Lemma schedule_wc_equation: *)
+  (*   forall G vars eq, *)
+  (*     wc_equation G vars eq -> *)
+  (*     wc_equation (schedule G) vars eq. *)
+  (* Proof. *)
+  (*   induction G as [|n G IH]; auto. *)
+  (*   intros vars eq Hwc. *)
+  (*   destruct eq; inv Hwc; eauto using wc_equation. *)
+  (*   econstructor; auto. *)
+  (*   - now eapply scheduler_find_node; eauto. *)
+  (*   - match goal with H:exists _, _ |- _ => *)
+  (*                     destruct H as (isub & osub & Hn_in & Hn_out) end. *)
+  (*     exists isub, osub. *)
+  (*     match goal with H:find_node _ _ = Some ?n0 |- _ => destruct n0 end; auto. *)
+  (* Qed. *)
+
+  (* Lemma scheduler_wc_global: *)
+  (*   forall G, *)
+  (*     wc_global G -> *)
+  (*     wc_global (schedule G). *)
+  (* Proof. *)
+  (*   intros G HG. *)
+  (*   induction G as [|n G Hwc IH]; auto. *)
+  (*   inversion HG as [|? G' WCG (WCi & WCo & WCv & WCeqs)]. subst. *)
+  (*   specialize (Hwc WCG). *)
+  (*   simpl. constructor; auto. *)
+  (*   destruct n. *)
+  (*   repeat (split; simpl; auto). *)
+  (*   rewrite schedule_eqs_permutation. *)
+  (*   apply Forall_impl with (2:=WCeqs). *)
+  (*   apply schedule_wc_equation. *)
+  (* Qed. *)
+
+
+  Lemma scheduler_initial_state:
+    forall S P b,
+      initial_state P b S ->
+      initial_state (schedule P) b S.
+  Proof.
+    induction S as [? IH] using memory_ind'.
+    inversion_clear 1 as [????? Find ? Insts].
+    apply scheduler_find_block in Find.
+    econstructor; eauto.
+    simpl; intros ** Hin.
+    apply Insts in Hin as (?&?&?).
+    eexists; intuition; eauto.
+  Qed.
+  Hint Resolve scheduler_initial_state.
+
+  Lemma scheduler_state_closed:
+    forall S P b,
+      state_closed P b S ->
+      state_closed (schedule P) b S.
+  Proof.
+    induction S as [? IH] using memory_ind'.
+    inversion_clear 1 as [????? Find ? Insts].
+    apply scheduler_find_block in Find.
+    econstructor; eauto.
+    simpl; intros ** Hin; pose proof Hin.
+    apply Insts in Hin as (?&?&?).
+    eexists; intuition; eauto.
+  Qed.
+  Hint Resolve scheduler_state_closed.
+
+  Lemma scheduler_transient_states_closed:
+    forall blocks P I,
+      transient_states_closed P blocks I ->
+      transient_states_closed (schedule P) blocks I.
+  Proof.
+    induction 1; constructor; auto.
+  Qed.
+  Hint Resolve scheduler_transient_states_closed.
+
+  Theorem scheduler_sem_block:
+    forall P b xs S S' ys,
+      sem_block P b xs S S' ys ->
+      sem_block (schedule P) b xs S S' ys.
+  Proof.
+    intro P;
+      induction 1 using sem_block_mult
+        with (P_equation := fun base R S I S' eq =>
+                              sem_equation (schedule P) base R S I S' eq);
+      eauto using sem_equation.
+    - econstructor; eauto.
+      cases; eauto.
+    - match goal with H: find_block _ _ = _ |- _ => apply scheduler_find_block in H end.
+      econstructor; eauto; simpl.
+      rewrite schedule_eqs_permutation; eauto.
+  Qed.
+
+End SBSCHEDULE.
+
+Module SBScheduleFun
+       (Ids    : IDS)
+       (Op     : OPERATORS)
+       (OpAux  : OPERATORS_AUX       Op)
+       (Clks   : CLOCKS          Ids)
+       (ExprSyn: NLEXPRSYNTAX        Op)
+       (Syn    : SBSYNTAX        Ids Op       Clks ExprSyn)
+       (Block  : SBISBLOCK       Ids Op       Clks ExprSyn Syn)
+       (Ord    : SBORDERED       Ids Op       Clks ExprSyn Syn Block)
+       (Str    : STREAM              Op OpAux)
+       (ExprSem: NLEXPRSEMANTICS Ids Op OpAux Clks ExprSyn               Str)
+       (Sem    : SBSEMANTICS     Ids Op OpAux Clks ExprSyn Syn Block Ord Str ExprSem)
+       (Sch    : EXT_NLSCHEDULER Ids Op       Clks ExprSyn Syn)
+<: SBSCHEDULE Ids Op OpAux Clks ExprSyn Syn Block Ord Str ExprSem Sem Sch.
+  Include SBSCHEDULE Ids Op OpAux Clks ExprSyn Syn Block Ord Str ExprSem Sem Sch.
+End SBScheduleFun.
